<?xml version="1.0" encoding="UTF-8"?>
<!--
  Licensed to the Apache Software Foundation (ASF) under one or more
  contributor license agreements.  See the NOTICE file distributed with
  this work for additional information regarding copyright ownership.
  The ASF licenses this file to You under the Apache License, Version 2.0
  (the "License"); you may not use this file except in compliance with
  the License.  You may obtain a copy of the License at

      http://www.apache.org/licenses/LICENSE-2.0

  Unless required by applicable law or agreed to in writing, software
  distributed under the License is distributed on an "AS IS" BASIS,
  WITHOUT WARRANTIES OR CONDITIONS OF ANY KIND, either express or implied.
  See the License for the specific language governing permissions and
  limitations under the License.
-->
<rdf:RDF
    xmlns:rdf="http://www.w3.org/1999/02/22-rdf-syntax-ns#"
    xmlns:protege="http://protege.stanford.edu/plugins/owl/protege#"
    xmlns:ep="http://stanbol.apache.org/ontology/enhancer/executionplan#"
    xmlns:owl="http://www.w3.org/2002/07/owl#"
    xmlns:xsd="http://www.w3.org/2001/XMLSchema#"
    xmlns="http://stanbol.apache.org/ontology/enhancer/executionmetadata#"
    xmlns:rdfs="http://www.w3.org/2000/01/rdf-schema#"
  xml:base="http://stanbol.apache.org/ontology/enhancer/executionmetadata">
  <owl:Ontology rdf:about="">
    <owl:imports rdf:resource="http://stanbol.apache.org/ontology/enhancer/executionplan"/>
    <rdfs:comment xml:lang="en">Allows to describe metadata about an actual execution of an EnhancementChain by the Stanbol Enhancer for a parsed ContentItem</rdfs:comment>
  </owl:Ontology>
  <owl:Class rdf:ID="ExecutionStatus">
    <rdfs:label rdf:datatype="http://www.w3.org/2001/XMLSchema#string"
    >Execution Status</rdfs:label>
    <rdfs:comment xml:lang="en">Class used to represent the status of an Execution</rdfs:comment>
  </owl:Class>
  <owl:Class rdf:ID="Execution">
    <rdfs:label xml:lang="en">Execution</rdfs:label>
    <rdfs:comment xml:lang="en">An execution (abstract)</rdfs:comment>
  </owl:Class>
  <owl:Class rdf:ID="ChainExecution">
    <rdfs:comment xml:lang="en">An execution of an EnhancementChain</rdfs:comment>
    <rdfs:subClassOf rdf:resource="#Execution"/>
    <rdfs:label xml:lang="en">EnhancementEngine Execution</rdfs:label>
  </owl:Class>
  <owl:Class rdf:ID="EngineExecution">
    <rdfs:label xml:lang="en">EnhancementEngine Execution</rdfs:label>
    <rdfs:comment xml:lang="en">An execution of an Enhancement Engine</rdfs:comment>
    <rdfs:subClassOf rdf:resource="#Execution"/>
  </owl:Class>
  <owl:DatatypeProperty rdf:ID="statusMessage">
    <rdfs:domain rdf:resource="#Execution"/>
    <rdfs:range rdf:resource="http://www.w3.org/2001/XMLSchema#string"/>
    <rdfs:label xml:lang="en">status message</rdfs:label>
    <rdfs:comment xml:lang="en">Allows to provide a status message for an execution (may be multi valued)</rdfs:comment>
  </owl:DatatypeProperty>
  <owl:DatatypeProperty rdf:ID="started">
    <rdfs:label xml:lang="en">started</rdfs:label>
    <rdfs:comment xml:lang="en">Time point when the exection started (also available when skipped)</rdfs:comment>
    <rdfs:range rdf:resource="http://www.w3.org/2001/XMLSchema#dateTime"/>
    <rdfs:domain rdf:resource="#Execution"/>
  </owl:DatatypeProperty>
  <owl:TransitiveProperty rdf:ID="executionPart">
    <rdf:type rdf:resource="http://www.w3.org/2002/07/owl#FunctionalProperty"/>
    <rdf:type rdf:resource="http://www.w3.org/2002/07/owl#ObjectProperty"/>
    <rdfs:comment xml:lang="en">Property that links an Execution to its parent ChainExecution (e.g. the Execution of single Engines to the Execution of the EnhancementChain)</rdfs:comment>
    <rdfs:range rdf:resource="#ChainExecution"/>
    <rdfs:domain rdf:resource="#Execution"/>
  </owl:TransitiveProperty>
  <owl:FunctionalProperty rdf:ID="enhancedBy">
    <rdf:type rdf:resource="http://www.w3.org/2002/07/owl#ObjectProperty"/>
    <rdfs:range rdf:resource="#ChainExecution"/>
    <rdf:type rdf:resource="http://www.w3.org/2002/07/owl#InverseFunctionalProperty"/>
    <rdfs:label xml:lang="en">enhanced by</rdfs:label>
    <owl:inverseOf>
      <owl:InverseFunctionalProperty rdf:ID="enhances"/>
    </owl:inverseOf>
    <rdfs:comment xml:lang="en">Property that links from the ContentItem to the ChainExecution (defining the root node of the execution metadata)</rdfs:comment>
  </owl:FunctionalProperty>
  <owl:FunctionalProperty rdf:ID="executionNode">
    <rdfs:domain rdf:resource="#EngineExecution"/>
    <rdfs:range rdf:resource="http://stanbol.apache.org/ontology/enhancer/executionplan#ExecutionNode"/>
    <rdf:type rdf:resource="http://www.w3.org/2002/07/owl#ObjectProperty"/>
    <rdfs:label xml:lang="en">execution node</rdfs:label>
    <rdfs:comment xml:lang="en">Property that links from the EngineExecution to the ExecutionNode of the ExecutionPlan</rdfs:comment>
  </owl:FunctionalProperty>
  <owl:FunctionalProperty rdf:ID="executionPlan">
    <rdfs:label xml:lang="en">execution plan</rdfs:label>
    <rdfs:comment xml:lang="en">Property that links from the ChainExecution to the ExecutionPlan.</rdfs:comment>
    <rdfs:domain rdf:resource="#ChainExecution"/>
    <rdfs:range rdf:resource="http://stanbol.apache.org/ontology/enhancer/executionplan#ExecutionPlan"/>
    <rdf:type rdf:resource="http://www.w3.org/2002/07/owl#ObjectProperty"/>
  </owl:FunctionalProperty>
  <owl:FunctionalProperty rdf:ID="status">
    <rdfs:comment xml:lang="en">The current/final status of an Execution. Allowed values are the instances of ExectionStatus defined by this Ontology</rdfs:comment>
    <rdfs:label xml:lang="en">status</rdfs:label>
    <rdfs:range rdf:resource="#ExecutionStatus"/>
    <rdfs:domain rdf:resource="#Execution"/>
    <rdf:type rdf:resource="http://www.w3.org/2002/07/owl#ObjectProperty"/>
  </owl:FunctionalProperty>
  <owl:FunctionalProperty rdf:ID="isDefaultChain">
    <rdfs:comment xml:lang="en">if the ChainExecution represents an execution of the default EnhancementChain of the Stanbol Enhancer.</rdfs:comment>
    <rdfs:range rdf:resource="http://www.w3.org/2001/XMLSchema#boolean"/>
    <rdfs:domain rdf:resource="#ChainExecution"/>
    <rdf:type rdf:resource="http://www.w3.org/2002/07/owl#DatatypeProperty"/>
    <rdfs:label xml:lang="en">is default Chain</rdfs:label>
  </owl:FunctionalProperty>
  <owl:FunctionalProperty rdf:ID="completed">
    <rdf:type rdf:resource="http://www.w3.org/2002/07/owl#DatatypeProperty"/>
    <rdfs:label xml:lang="en">completed</rdfs:label>
    <rdfs:comment xml:lang="en">time point when the execution completed (succeded, skipped or failed).</rdfs:comment>
    <rdfs:range rdf:resource="http://www.w3.org/2001/XMLSchema#dateTime"/>
    <rdfs:domain rdf:resource="#Execution"/>
  </owl:FunctionalProperty>
  <owl:InverseFunctionalProperty rdf:about="#enhances">
    <rdf:type rdf:resource="http://www.w3.org/2002/07/owl#FunctionalProperty"/>
    <rdf:type rdf:resource="http://www.w3.org/2002/07/owl#ObjectProperty"/>
    <rdfs:label xml:lang="en">enhances</rdfs:label>
    <rdfs:comment xml:lang="en">Property that links from the ChainExecution to the enhanced ContentItem</rdfs:comment>
    <rdfs:domain rdf:resource="#ChainExecution"/>
    <owl:inverseOf rdf:resource="#enhancedBy"/>
  </owl:InverseFunctionalProperty>
  <ExecutionStatus rdf:ID="StatusInProgress">
    <rdfs:comment xml:lang="en">ExecutionStatus indicating that the execution is in progress</rdfs:comment>
    <rdfs:label xml:lang="en">in progress</rdfs:label>
  </ExecutionStatus>
  <ExecutionStatus rdf:ID="StatusSkipped">
    <rdfs:label xml:lang="en">skipped</rdfs:label>
    <rdfs:comment xml:lang="en">ExecutionStatus indicating that the execution was skipped</rdfs:comment>
  </ExecutionStatus>
  <ExecutionStatus rdf:ID="StatusSheduled">
    <rdfs:label rdf:datatype="http://www.w3.org/2001/XMLSchema#string"
    >sheduled</rdfs:label>
    <rdfs:comment xml:lang="en">ExecutionStatus indicating that the execution is scheduled, but has not yet started</rdfs:comment>
  </ExecutionStatus>
  <ExecutionStatus rdf:ID="StatusCompleted">
    <rdfs:label xml:lang="en">completed</rdfs:label>
    <rdfs:comment xml:lang="en">ExecutionStatus indicating that the execution has completed successfully</rdfs:comment>
  </ExecutionStatus>
  <ExecutionStatus rdf:ID="StatusFailed">
    <rdfs:comment xml:lang="en">ExecutionStatus indicating that the execution has failed</rdfs:comment>
    <rdfs:label rdf:datatype="http://www.w3.org/2001/XMLSchema#string"
    >failed</rdfs:label>
  </ExecutionStatus>
</rdf:RDF>